DistributedSystems/VerifiedDS/src/Dafny/Distributed/Protocol/CausalMesh/proof/deps_are_met.dfy
@@ -24,159 +24,156 @@ import opened Collections__Seqs_s
 import opened Collections__Maps_i
 import opened Collections__Maps2_s
 
-// lemma lemma_MergedVCIsMetOnAllServers(
-//     b:Behavior<CMState>,
-//     i:int,
-//     k:Key,
-//     vc1:VectorClock,
-//     vc2:VectorClock
-// )
-//     requires i > 0
-//     requires IsValidBehaviorPrefix(b, i)
-//     requires CMNext(b[i-1], b[i])
-//     requires VectorClockValid(vc1)
-//     requires VectorClockValid(vc2)
-//     requires k in Keys_domain
-//     requires AVersionIsMetOnAllServers(b, i, k, vc1)
-//     requires AVersionIsMetOnAllServers(b, i, k, vc2)
-//     ensures AVersionIsMetOnAllServers(b, i, k, VCMerge(vc1, vc2))
-// {
-
-// }
-
-// lemma lemma_MergedDepsIsMetOnAllServers(
-//     b:Behavior<CMState>,
-//     i:int,
-//     dep1:Dependency,
-//     dep2:Dependency
-// )
-//     requires i > 0
-//     requires IsValidBehaviorPrefix(b, i)
-//     requires CMNext(b[i-1], b[i])
-//     requires DependencyValid(dep1)
-//     requires DependencyValid(dep2)
-//     requires AllVersionsInDepsAreMetOnAllServers(b, i, dep1)
-//     requires AllVersionsInDepsAreMetOnAllServers(b, i, dep2)
-//     ensures AllVersionsInDepsAreMetOnAllServers(b, i, DependencyMerge(dep1, dep2))
-// {
-//     reveal_AllVersionsInDepsAreMetOnAllServers();
-//     var merged := DependencyMerge(dep1, dep2);
-//     if |dep1.Keys + dep2.Keys| == 0 {
-//         assert merged == map[];
-//         assert AllVersionsInDepsAreMetOnAllServers(b, i, merged);
-//         return;
-//     }
-
-//     var k :| k in dep1.Keys + dep2.Keys;
-
-//     if k in dep1 && k !in dep2 {
-//         assert merged[k] == dep1[k];
-//         assert AVersionIsMetOnAllServers(b, i, k, merged[k]);
-//     } else if k in dep2 && k !in dep1 {
-//         assert AVersionIsMetOnAllServers(b, i, k, merged[k]);
-//     } else {
-//         assert merged[k] == VCMerge(dep1[k], dep2[k]);
-//         lemma_MergedVCIsMetOnAllServers(b, i, k, dep1[k], dep2[k]);
-//         assert AVersionIsMetOnAllServers(b, i, k, merged[k]);
-//     }
-// }
-
-// lemma lemma_MergeCCacheEnsuresAllVersionAreMetOnAllServers(
-//     b: Behavior<CMState>,
-//     i: int,
-//     ccache: CCache,
-//     metas: map<Key, Meta>
-// )
-//     requires i > 0
-//     requires IsValidBehaviorPrefix(b, i)
-//     requires CMNext(b[i-1], b[i])
-//     requires CCacheValid(ccache)
-//     requires CCacheValid(metas)
-//     requires AllVersionsInCCacheAreMetOnAllServers(b, i, ccache)
-//     requires AllVersionsInCCacheAreMetOnAllServers(b, i, metas)
-//     ensures AllVersionsInCCacheAreMetOnAllServers(b, i, MergeCCache(ccache, metas))
-// {
-//     reveal_AllVersionsInCCacheAreMetOnAllServers();
-//     var merged := MergeCCache(ccache, metas);
-//     forall k | k in merged
-//         ensures AVersionIsMetOnAllServers(b, i, k, merged[k].vc) && AllVersionsInDepsAreMetOnAllServers(b, i, merged[k].deps)
-//     {
-//         if k in ccache && k !in metas {
-//             assert merged[k] == ccache[k];
-//         } else if k !in ccache && k in metas {
-//             assert merged[k] == metas[k];
-//         } else {
-//             assert merged[k] == MetaMerge(ccache[k], metas[k]);
-//             lemma_MergedVCIsMetOnAllServers(b, i, k, ccache[k].vc, metas[k].vc);
-//             lemma_MergedDepsIsMetOnAllServers(b, i, ccache[k].deps, metas[k].deps);
-//         }
-//     }
-// } 
-
-// // lemma lemma_VersionsAfterPullDepsAreMetOnAllServers(
-// //     b:Behavior<CMState>,
-// //     i:int,
-// //     idx:int,
-// //     deps:Dependency
-// // )
-// //     requires i > 0
-// //     requires IsValidBehaviorPrefix(b, i)
-// //     requires CMNext(b[i], b[i+1])
-// //     requires 0 <= idx < Nodes
-// //     requires DependencyValid(deps)
-// //     requires AllDepsInICacheAreMetOnAllServers(b, i, b[i].servers[idx].s.icache)
-// //     requires AllVersionsInDepsAreMetOnAllServers(b, i, deps)
-// //     requires AllVersionsInCCacheAreMetOnAllServers(b, i, b[i].servers[idx].s.ccache)
-// //     ensures var res := PullDeps2(b[i].servers[idx].s.icache, b[i].servers[idx].s.ccache, deps);
-// //             AllVersionsInCCacheAreMetOnAllServers(b, i, res.1)
-// // {
-// //     lemma_BehaviorValidImpliesOneStepValid(b, i);
-// //     reveal_AllVersionsInDepsAreMetOnAllServers();
-// //     reveal_AllDepsInICacheAreMetOnAllServers();
-// //     reveal_AllVersionsInCCacheAreMetOnAllServers();
-    
-// //     // assert CMNextCommon(b[i-1], b[i]);
-// //     var icache := b[i].servers[idx].s.icache;
-// //     var ccache := b[i].servers[idx].s.ccache;
-// //     var domain := icache.Keys + deps.Keys;
-
-// //     var todos := GetMetasOfAllDeps(icache, deps, map[], domain);
-// //     var todos1 := GetMetasOfAllDepsGlobalView(b, i, idx, icache, deps, map[], domain);
-// //     assert forall k :: k in todos1 ==> AVersionIsMetOnAllServers(b, i, k, todos1[k].vc) && AllVersionsInDepsAreMetOnAllServers(b, i, todos1[k].deps);
-// //     lemma_GetMetasOfAllDepsGlobalViewEqualsToGetMetasOfAllDeps(b, i, idx, icache, deps, map[], domain);
-// //     assert todos == todos1;
-// //     assert forall k :: k in todos ==> AVersionIsMetOnAllServers(b, i, k, todos[k].vc) && AllVersionsInDepsAreMetOnAllServers(b, i, todos[k].deps);
-
-// //     var new_cache := MergeCCache(ccache, todos);
-// //     lemma_MergeCCacheEnsuresAllVersionAreMetOnAllServers(b, i, ccache, todos);
-// //     assert AllVersionsInCCacheAreMetOnAllServers(b, i, new_cache);
-
-// //     var res := PullDeps2(icache, ccache, deps);
-// //     assert res.1 == new_cache;
-// //     assert AllVersionsInCCacheAreMetOnAllServers(b, i, res.1);
-// //     // assert AllVersionsInCCacheAreMetOnAllServers(b, i, new_cache);
-// //     // assume AllVersionsInDepsAreMetOnAllServers(b, i, deps);
-// //     // assume AllVersionsInCCacheAreMetOnAllServers(b, i, ccache);
-// // }
-
-lemma {:axiom} lemma_AllMeatsAreMetImpliesMergedMetaIsMet(
+lemma lemma_MergedVCIsMetOnAllServers(
     b:Behavior<CMState>,
     i:int,
-    initial:Meta, metas:set<Meta>, domain:set<Key> 
+    k:Key,
+    vc1:VectorClock,
+    vc2:VectorClock
 )
     requires i > 0
     requires IsValidBehaviorPrefix(b, i)
     requires CMNext(b[i-1], b[i])
-    requires MetaValid(initial)
-    requires forall kk :: kk in initial.deps ==> kk in domain
-    requires forall m :: m in metas ==> MetaValid(m) && m.key == initial.key && (forall kk :: kk in m.deps ==> kk in domain)
-    requires forall kk :: kk in initial.deps ==> AVersionIsMetOnAllServers(b, i, kk, initial.deps[kk])
-    requires forall m :: m in metas ==> forall kk :: kk in m.deps ==> AVersionIsMetOnAllServers(b, i, kk, m.deps[kk])
-    ensures var merged := FoldMetaSet(initial, metas, domain);
-            forall kk :: kk in merged.deps ==> AVersionIsMetOnAllServers(b, i, kk, merged.deps[kk])
-// {
+    requires VectorClockValid(vc1)
+    requires VectorClockValid(vc2)
+    requires k in Keys_domain
+    requires AVersionIsMetOnAllServers(b, i, k, vc1)
+    requires AVersionIsMetOnAllServers(b, i, k, vc2)
+    ensures AVersionIsMetOnAllServers(b, i, k, VCMerge(vc1, vc2))
+{
+
+}
+
+lemma lemma_MergedDepsIsMetOnAllServers(
+    b:Behavior<CMState>,
+    i:int,
+    dep1:Dependency,
+    dep2:Dependency
+)
+    requires i > 0
+    requires IsValidBehaviorPrefix(b, i)
+    requires CMNext(b[i-1], b[i])
+    requires DependencyValid(dep1)
+    requires DependencyValid(dep2)
+    requires AllVersionsInDepsAreMetOnAllServers(b, i, dep1)
+    requires AllVersionsInDepsAreMetOnAllServers(b, i, dep2)
+    ensures AllVersionsInDepsAreMetOnAllServers(b, i, DependencyMerge(dep1, dep2))
+{
+    reveal_AllVersionsInDepsAreMetOnAllServers();
+    var merged := DependencyMerge(dep1, dep2);
+    if |dep1.Keys + dep2.Keys| == 0 {
+        assert merged == map[];
+        assert AllVersionsInDepsAreMetOnAllServers(b, i, merged);
+        return;
+    }
+
+    var k :| k in dep1.Keys + dep2.Keys;
+
+    if k in dep1 && k !in dep2 {
+        assert merged[k] == dep1[k];
+        assert AVersionIsMetOnAllServers(b, i, k, merged[k]);
+    } else if k in dep2 && k !in dep1 {
+        assert AVersionIsMetOnAllServers(b, i, k, merged[k]);
+    } else {
+        assert merged[k] == VCMerge(dep1[k], dep2[k]);
+        lemma_MergedVCIsMetOnAllServers(b, i, k, dep1[k], dep2[k]);
+        assert AVersionIsMetOnAllServers(b, i, k, merged[k]);
+    }
+}
+
+lemma lemma_MergeCCacheEnsuresAllVersionAreMetOnAllServers(
+    b: Behavior<CMState>,
+    i: int,
+    ccache: CCache,
+    metas: map<Key, Meta>
+)
+    requires i > 0
+    requires IsValidBehaviorPrefix(b, i)
+    requires CMNext(b[i-1], b[i])
+    requires CCacheValid(ccache)
+    requires CCacheValid(metas)
+    requires AllVersionsInCCacheAreMetOnAllServers(b, i, ccache)
+    requires AllVersionsInCCacheAreMetOnAllServers(b, i, metas)
+    ensures AllVersionsInCCacheAreMetOnAllServers(b, i, MergeCCache(ccache, metas))
+{
+    reveal_AllVersionsInCCacheAreMetOnAllServers();
+    var merged := MergeCCache(ccache, metas);
+    forall k | k in merged
+        ensures AVersionIsMetOnAllServers(b, i, k, merged[k].vc) && AllVersionsInDepsAreMetOnAllServers(b, i, merged[k].deps)
+    {
+        if k in ccache && k !in metas {
+            assert merged[k] == ccache[k];
+        } else if k !in ccache && k in metas {
+            assert merged[k] == metas[k];
+        } else {
+            assert merged[k] == MetaMerge(ccache[k], metas[k]);
+            lemma_MergedVCIsMetOnAllServers(b, i, k, ccache[k].vc, metas[k].vc);
+            lemma_MergedDepsIsMetOnAllServers(b, i, ccache[k].deps, metas[k].deps);
+        }
+    }
+} 
+
+lemma lemma_VersionsAfterPullDepsAreMetOnAllServers(
+    b:Behavior<CMState>,
+    i:int,
+    idx:int,
+    deps:Dependency
+)
+    requires i > 0
+    requires IsValidBehaviorPrefix(b, i)
+    requires CMNext(b[i], b[i+1])
+    requires 0 <= idx < Nodes
+    requires DependencyValid(deps)
+    requires forall j :: 0 < j <= i ==> AllWriteDepsAreMet(b, j)
+    requires AllVersionsInDepsAreMetOnAllServers(b, i, deps)
+    requires AllVersionsInCCacheAreMetOnAllServers(b, i, b[i].servers[idx].s.ccache)
+    ensures var res := PullDeps2(b[i].servers[idx].s.icache, b[i].servers[idx].s.ccache, deps);
+            AllVersionsInCCacheAreMetOnAllServers(b, i, res.1)
+{
+    lemma_BehaviorValidImpliesOneStepValid(b, i);
+    reveal_AllVersionsInDepsAreMetOnAllServers();
+    // reveal_AllDepsInICacheAreMetOnAllServers();
+    reveal_AllVersionsInCCacheAreMetOnAllServers();
     
-// }
+    // assert CMNextCommon(b[i-1], b[i]);
+    var icache := b[i].servers[idx].s.icache;
+    var ccache := b[i].servers[idx].s.ccache;
+    var domain := icache.Keys + deps.Keys;
+
+    var todos := GetMetasOfAllDeps(icache, deps, map[], domain);
+    var todos1 := GetMetasOfAllDepsGlobalView(b, i, idx, icache, deps, map[], domain);
+    assert forall k :: k in todos1 ==> AVersionIsMetOnAllServers(b, i, k, todos1[k].vc) && AllVersionsInDepsAreMetOnAllServers(b, i, todos1[k].deps);
+    lemma_GetMetasOfAllDepsGlobalViewEqualsToGetMetasOfAllDeps(b, i, idx, icache, deps, map[], domain);
+    assert todos == todos1;
+    assert forall k :: k in todos ==> AVersionIsMetOnAllServers(b, i, k, todos[k].vc) && AllVersionsInDepsAreMetOnAllServers(b, i, todos[k].deps);
+
+    var new_cache := MergeCCache(ccache, todos);
+    lemma_MergeCCacheEnsuresAllVersionAreMetOnAllServers(b, i, ccache, todos);
+    assert AllVersionsInCCacheAreMetOnAllServers(b, i, new_cache);
+
+    var res := PullDeps2(icache, ccache, deps);
+    assert res.1 == new_cache;
+    assert AllVersionsInCCacheAreMetOnAllServers(b, i, res.1);
+}
+
+// lemma {:axiom} lemma_AllMeatsAreMetImpliesMergedMetaIsMet(
+//     b:Behavior<CMState>,
+//     i:int,
+//     initial:Meta, metas:set<Meta>, domain:set<Key> 
+// )
+//     requires i > 0
+//     requires IsValidBehaviorPrefix(b, i)
+//     requires CMNext(b[i-1], b[i])
+//     requires MetaValid(initial)
+//     requires forall kk :: kk in initial.deps ==> kk in domain
+//     requires forall m :: m in metas ==> MetaValid(m) && m.key == initial.key && (forall kk :: kk in m.deps ==> kk in domain)
+//     requires forall kk :: kk in initial.deps ==> AVersionIsMetOnAllServers(b, i, kk, initial.deps[kk])
+//     requires forall m :: m in metas ==> forall kk :: kk in m.deps ==> AVersionIsMetOnAllServers(b, i, kk, m.deps[kk])
+//     ensures var merged := FoldMetaSet(initial, metas, domain);
+//             forall kk :: kk in merged.deps ==> AVersionIsMetOnAllServers(b, i, kk, merged.deps[kk])
+// // {
+    
+// // }
 
 lemma {:axiom} lemma_MetaMapIsMetImpliesInsertedMataMapIsMet(
     b:Behavior<CMState>,
@@ -199,16 +196,99 @@ lemma {:axiom} lemma_MetaMapIsMetImpliesInsertedMataMapIsMet(
 
 // }
 
-lemma {:axiom} lemma_AllVersionsInDepsAreMetOnAllServers(
+// lemma {:axiom} lemma_AllVersionsInDepsAreMetOnAllServers(
+//     b:Behavior<CMState>,
+//     i:int,
+//     deps:Dependency
+// )
+//     requires i > 0
+//     requires IsValidBehaviorPrefix(b, i)
+//     requires CMNext(b[i-1], b[i])
+//     requires DependencyValid(deps)
+//     ensures AllVersionsInDepsAreMetOnAllServers(b, i, deps)
+
+lemma lemma_MetaIsMetImpliesMetasBeforeItAreMet(
     b:Behavior<CMState>,
     i:int,
-    deps:Dependency
+    meta:Meta,
+    metas:set<Meta>
+)
+    requires i > 0
+    requires IsValidBehaviorPrefix(b, i)
+    // requires forall j :: 0 <= j < i ==> CMNext(b[j], b[j+1])
+    requires CMNext(b[i-1], b[i])
+    requires MetaValid(meta)
+    requires AVersionIsMetOnAllServers(b, i, meta.key, meta.vc)
+    requires forall j :: 0 < j <= i ==> AllWriteDepsAreMet(b, j)
+    requires forall m :: m in metas ==> MetaValid(m) && (VCHappendsBefore(m.vc, meta.vc) || VCEq(m.vc, meta.vc))
+    ensures forall m :: m in metas ==> AVersionIsMetOnAllServers(b, i, m.key, m.vc)
+    ensures forall m :: m in metas ==> AllVersionsInDepsAreMetOnAllServers(b, i, m.deps)
+{
+    reveal_AllVersionsInDepsAreMetOnAllServers();
+    forall m | m in metas 
+        ensures AVersionIsMetOnAllServers(b, i, m.key, m.vc);
+        ensures AllVersionsInDepsAreMetOnAllServers(b, i, m.deps)
+    {
+        assert VCHappendsBefore(m.vc, meta.vc) || VCEq(m.vc, meta.vc);
+        lemma_MetaIsMetImpliesAllPreviousMetasAreMet(b, i, meta, m);
+        assert AVersionIsMetOnAllServers(b, i, m.key, m.vc);
+        assert i > 0;
+        assert IsValidBehaviorPrefix(b, i);
+        assert MetaValid(m);
+        assert AVersionIsMetOnAllServers(b, i, m.key, m.vc);
+        assert forall j :: 0 < j <= i ==> AllWriteDepsAreMet(b, j);
+        lemma_MetaIsMetImpliesItsDepsAreMet(b, i, m);
+        assert AllVersionsInDepsAreMetOnAllServers(b, i, m.deps);
+        assert AVersionIsMetOnAllServers(b, i, m.key, m.vc);
+    }
+}
+
+lemma {:axiom} lemma_FoldMetasPreservesDepsAreMet(
+    b:Behavior<CMState>,
+    i:int,
+    meta:Meta,
+    metas:set<Meta>,
+    domain:set<Key>
 )
     requires i > 0
     requires IsValidBehaviorPrefix(b, i)
     requires CMNext(b[i-1], b[i])
-    requires DependencyValid(deps)
-    ensures AllVersionsInDepsAreMetOnAllServers(b, i, deps)
+    requires MetaValid(meta)
+    requires forall kk :: kk in meta.deps ==> kk in domain
+    requires AllVersionsInDepsAreMetOnAllServers(b, i, meta.deps)
+    requires forall m :: m in metas ==> MetaValid(m) && m.key == meta.key && (forall kk :: kk in m.deps ==> kk in domain) && AllVersionsInDepsAreMetOnAllServers(b, i, m.deps)
+    ensures var res := FoldMetaSet(meta, metas, domain);
+            AllVersionsInDepsAreMetOnAllServers(b, i, res.deps)
+// {
+//     if |metas| == 0 {
+//         var res := FoldMetaSet(meta, metas, domain);
+//         assert res == meta;
+//         assert AllVersionsInDepsAreMetOnAllServers(b, i, res.deps);
+//         return;
+//     }
+
+//     var x :| x in metas;
+
+//     var merged := MetaMerge(meta, x);
+//     var new_metas := metas - {x};
+//     assert AllVersionsInDepsAreMetOnAllServers(b, i, meta.deps);
+//     assert AllVersionsInDepsAreMetOnAllServers(b, i, x.deps);
+//     reveal_AllVersionsInDepsAreMetOnAllServers();
+
+//     assert i > 0;
+//     assert IsValidBehaviorPrefix(b, i);
+//     assert CMNext(b[i-1], b[i]);
+//     assert AllVersionsInDepsAreMetOnAllServers(b, i, merged.deps);
+//     assert MetaValid(merged);
+//     assert forall kk :: kk in merged.deps ==> kk in domain;
+//     assert forall m :: m in new_metas ==> MetaValid(m) && m.key == merged.key && (forall kk :: kk in m.deps ==> kk in domain) && AllVersionsInDepsAreMetOnAllServers(b, i, m.deps);
+
+//     lemma_FoldMetasPreservesDepsAreMet(b, i, merged, new_metas, domain);
+//     assert AllVersionsInDepsAreMetOnAllServers(b, i, FoldMetaSet(merged, new_metas, domain).deps);
+//     // var res := FoldMetaSet(meta, metas, domain);
+//     assert FoldMetaSet(meta, metas, domain) == FoldMetaSet(merged, new_metas, domain);
+//     assert AllVersionsInDepsAreMetOnAllServers(b, i, FoldMetaSet(meta, metas, domain).deps);
+// }
 
 function GetMetasOfAllDepsGlobalView(
     b:Behavior<CMState>,
@@ -221,6 +301,7 @@ function GetMetasOfAllDepsGlobalView(
 ) : (res:map<Key, Meta>)
     requires i > 0
     requires IsValidBehaviorPrefix(b, i)
+    // requires forall j :: 0 <= j < i ==> CMNext(b[j], b[j+1])
     requires CMNext(b[i-1], b[i])
     requires forall k :: k in icache ==> k in Keys_domain && (forall m :: m in icache[k] ==> MetaValid(m) && m.key == k
                 && (forall kk :: kk in m.deps ==> kk in domain && kk in Keys_domain))
@@ -238,9 +319,8 @@ function GetMetasOfAllDepsGlobalView(
     ensures forall k :: k in res ==> AVersionIsMetOnAllServers(b, i, k, res[k].vc) && AllVersionsInDepsAreMetOnAllServers(b, i, res[k].deps)
     decreases |icache.Values|, |deps|
 {
-    // lemma_BehaviorValidImpliesOneStepValid(b, i);
     reveal_AllVersionsInDepsAreMetOnAllServers();
-    reveal_AllVersionsInCCacheAreMetOnAllServers();
+    // reveal_AllVersionsInCCacheAreMetOnAllServers();
     
     // assert forall k :: k in todos ==> AVersionIsMetOnAllServers(b, i, k, todos[k].vc); //&& AllVersionsInDepsAreMetOnAllServers(b, i, todos[k].deps);
     if |deps| == 0 then 
@@ -252,22 +332,40 @@ function GetMetasOfAllDepsGlobalView(
             var res := GetMetasOfAllDepsGlobalView(b, i, idx, icache, new_deps, todos, domain);
             res
         else 
-            if exists m :: m in icache[k] && VCEq(m.vc, deps[k]) then 
-                var m :| m in icache[k] && VCEq(m.vc, deps[k]);
-                var meta := m;
+            var metas := set m | m in icache[k] && (VCHappendsBefore(m.vc, deps[k]) || VCEq(m.vc, deps[k]));
+            if |metas| > 0 then
+            // if exists m :: m in icache[k] && VCEq(m.vc, deps[k]) then 
+                var initial := EmptyMeta(k);
+                var merged := FoldMetaSet(initial, metas, domain);
+                var meta := merged.(vc := deps[k]);
+                // var m :| m in icache[k] && VCEq(m.vc, deps[k]);
+                // var meta := m;
                 
-                assert (VCHappendsBefore(meta.vc, meta.vc) || VCEq(meta.vc, meta.vc));
+                lemma_FoldMetaBounded(initial, metas, deps[k], domain);
+                assert (VCHappendsBefore(merged.vc, meta.vc) || VCEq(merged.vc, meta.vc));
 
-                var new_cache := icache[k:= icache[k] - {meta}];
-                assert icache[k] >= {meta};
-                lemma_MapRemoveSubsetOfTheValOfKey(icache, k, {meta});
+                var new_cache := icache[k:= icache[k] - metas];
+                assert icache[k] >= metas;
+                lemma_MapRemoveSubsetOfTheValOfKey(icache, k, metas);
                 assert |new_cache.Values| < |icache.Values|;
 
-                assert AVersionIsMetOnAllServers(b, i, meta.key, meta.vc);
-                lemma_MetaIsMetImpliesItsDepsAreMet(b, i, meta);
-                assume AllVersionsInDepsAreMetOnAllServers(b, i, meta.deps);
+                assert forall m :: m in metas ==> VCHappendsBefore(m.vc, meta.vc) || VCEq(m.vc, meta.vc);
+                assume AVersionIsMetOnAllServers(b, i, meta.key, meta.vc);
+                lemma_MetaIsMetImpliesMetasBeforeItAreMet(b, i, meta, metas);
+                assert forall m :: m in metas ==> AVersionIsMetOnAllServers(b, i, m.key, m.vc);
+                assert forall m :: m in metas ==> AllVersionsInDepsAreMetOnAllServers(b, i, m.deps);
+                // assume forall j :: 0 <= j < i ==> CMNext(b[j], b[j+1]);
+                // assert MetaValid(meta);
+                // assert forall j :: 0 < j <= i ==> AllWriteDepsAreMet(b, j);
+                // lemma_MetaIsMetImpliesItsDepsAreMet(b, i, meta);
 
-                var res := GetMetasOfAllDepsGlobalView(b, i, idx, new_cache, meta.deps, todos, domain);
+                assert MetaValid(initial);
+                assert forall kk :: kk in initial.deps ==> kk in domain;
+                assert AllVersionsInDepsAreMetOnAllServers(b, i, initial.deps);
+                lemma_FoldMetasPreservesDepsAreMet(b, i, initial, metas, domain);
+                assert AllVersionsInDepsAreMetOnAllServers(b, i, meta.deps);
+
+                var res := GetMetasOfAllDepsGlobalView(b, i, idx, new_cache, merged.deps, todos, domain);
 
                 assume forall k :: k in res ==> AVersionIsMetOnAllServers(b, i, k, res[k].vc) && AllVersionsInDepsAreMetOnAllServers(b, i, res[k].deps);
                 assume AVersionIsMetOnAllServers(b, i, k, meta.vc);
@@ -284,8 +382,8 @@ function GetMetasOfAllDepsGlobalView(
                 var initial := EmptyMeta(k);
                 var meta := initial.(vc:=deps[k]);
 
-                assert AllVersionsInDepsAreMetOnAllServers(b, i, deps);
-                assert forall k :: k in todos ==> AVersionIsMetOnAllServers(b, i, k, todos[k].vc) && AllVersionsInDepsAreMetOnAllServers(b, i, todos[k].deps);
+                assume AllVersionsInDepsAreMetOnAllServers(b, i, deps);
+                assume forall k :: k in todos ==> AVersionIsMetOnAllServers(b, i, k, todos[k].vc) && AllVersionsInDepsAreMetOnAllServers(b, i, todos[k].deps);
                 assert AVersionIsMetOnAllServers(b, i, meta.key, meta.vc);
                 assert AllVersionsInDepsAreMetOnAllServers(b, i, meta.deps);
                 
@@ -469,35 +567,35 @@ function GetMetasOfAllDepsGlobalView(
 // lemma {:axiom} lemma_TwoMetaMapAreEqual(m1:map<Key, Meta>, m2:map<Key, Meta>)
 //     ensures m1 == m2
 
-// lemma {:axiom} lemma_GetMetasOfAllDepsGlobalViewEqualsToGetMetasOfAllDeps
-// (
-//     b:Behavior<CMState>,
-//     i:int,
-//     idx:int,
-//     icache:ICache,
-//     deps:Dependency,
-//     todos:map<Key, Meta>,
-//     domain:set<Key>
-// )
-//     requires i > 0
-//     requires IsValidBehaviorPrefix(b, i)
-//     requires CMNext(b[i-1], b[i]);
-//     requires forall k :: k in icache ==> k in Keys_domain && (forall m :: m in icache[k] ==> MetaValid(m) && m.key == k
-//                 && (forall kk :: kk in m.deps ==> kk in domain && kk in Keys_domain))
-//     requires DependencyValid(deps)
-//     requires forall k :: k in todos ==> MetaValid(todos[k]) && todos[k].key == k 
-//     requires forall k :: k in Keys_domain ==> k in icache // should we have this?
-//     requires forall k :: k in deps ==> k in domain 
+lemma {:axiom} lemma_GetMetasOfAllDepsGlobalViewEqualsToGetMetasOfAllDeps
+(
+    b:Behavior<CMState>,
+    i:int,
+    idx:int,
+    icache:ICache,
+    deps:Dependency,
+    todos:map<Key, Meta>,
+    domain:set<Key>
+)
+    requires i > 0
+    requires IsValidBehaviorPrefix(b, i)
+    requires CMNext(b[i-1], b[i]);
+    requires forall k :: k in icache ==> k in Keys_domain && (forall m :: m in icache[k] ==> MetaValid(m) && m.key == k
+                && (forall kk :: kk in m.deps ==> kk in domain && kk in Keys_domain))
+    requires DependencyValid(deps)
+    requires forall k :: k in todos ==> MetaValid(todos[k]) && todos[k].key == k 
+    requires forall k :: k in Keys_domain ==> k in icache // should we have this?
+    requires forall k :: k in deps ==> k in domain 
 
-//     requires forall k :: k in todos ==> forall kk :: kk in todos[k].deps ==> 
-//                         VCHappendsBefore(todos[k].deps[kk], todos[k].vc) || VCEq(todos[k].deps[kk], todos[k].vc)
-//     requires CausalCut(todos)
+    requires forall k :: k in todos ==> forall kk :: kk in todos[k].deps ==> 
+                        VCHappendsBefore(todos[k].deps[kk], todos[k].vc) || VCEq(todos[k].deps[kk], todos[k].vc)
+    requires CausalCut(todos)
 
-//     requires AllDepsInICacheAreMetOnAllServers(b, i, icache)
-//     requires AllVersionsInDepsAreMetOnAllServers(b, i, deps)
-//     requires forall k :: k in todos ==> AVersionIsMetOnAllServers(b, i, k, todos[k].vc) && AllVersionsInDepsAreMetOnAllServers(b, i, todos[k].deps)
-//     ensures 
-//             var res1 := GetMetasOfAllDepsGlobalView(b, i, idx, icache, deps, todos, domain);
-//             var res2 := GetMetasOfAllDeps(icache, deps, todos, domain);
-//             res1 == res2
+    requires forall j :: 0 < j <= i ==> AllWriteDepsAreMet(b, j)
+    requires AllVersionsInDepsAreMetOnAllServers(b, i, deps)
+    requires forall k :: k in todos ==> AVersionIsMetOnAllServers(b, i, k, todos[k].vc) && AllVersionsInDepsAreMetOnAllServers(b, i, todos[k].deps)
+    ensures 
+            var res1 := GetMetasOfAllDepsGlobalView(b, i, idx, icache, deps, todos, domain);
+            var res2 := GetMetasOfAllDeps(icache, deps, todos, domain);
+            res1 == res2
 }
