DistributedSystems/VerifiedDS/src/Dafny/Distributed/Protocol/CausalMesh/proof/propagation.dfy
@@ -2,7 +2,7 @@ include "../distributed_system.dfy"
 // include "causalcut.dfy"
 include "packet_sending.dfy"
 include "properties.dfy"
-include "propagation_lemma.dfy"
+include "propagation_lemma2.dfy"
 include "../../../Common/Collections/Seqs.s.dfy"
 
 module CausalMesh_Proof_Propagation_i {
@@ -16,7 +16,7 @@ import opened CausalMesh_Proof_Actions_i
 import opened Temporal__Temporal_s
 import opened CausalMesh_proof_Assumptions_i
 import opened CausalMesh_Proof_Constants_i
-import opened CausalMesh_Proof_PropagationLemma_i
+import opened CausalMesh_Proof_PropagationLemma2_i
 import opened CausalMesh_Proof_PacketSending_i
 import opened CausalMesh_Proof_Properties_i
 // import opened CausalMesh_Proof_MessageReadReply_i
@@ -34,11 +34,11 @@ lemma lemma_PropagationAtTail(
 )
     requires 0 < i 
     requires IsValidBehaviorPrefix(b, i)
-    requires forall j :: 0 <= j < i ==> CMNext(b[j], b[j+1])
+    // requires forall j :: 0 <= j < i ==> CMNext(b[j], b[j+1])
     requires CMNext(b[i-1], b[i])
     requires forall j :: 0 < j <= i ==> AllWriteDepsAreMet(b, j)
     requires 0 <= idx < Nodes
-    requires |ios| > 1
+    requires |ios| > 0
     requires ios[0].LIoOpReceive?
     requires p.msg.Message_Propagation?
     requires p in b[i-1].environment.sentPackets
@@ -47,6 +47,7 @@ lemma lemma_PropagationAtTail(
     requires ios[0].r == p
     requires PacketValid(p)
     requires p.msg.start == b[i-1].servers[idx].s.next
+    requires p.msg.round == 2
     requires ReceivePropagate(b[i-1].servers[idx].s, b[i].servers[idx].s, p, ExtractSentPacketsFromIos(ios))
     ensures AVersionIsMetOnAllServers(b, i, ios[0].r.msg.key, ios[0].r.msg.meta.vc)
 {
@@ -68,7 +69,7 @@ lemma lemma_PropagationAtTail(
     assert PacketValid(p);
 
     assert p.dst == idx;
-    assert idx == s.id;
+    // assert idx == s.id;
 
     var nodes := lemma_Propagation2(b, i-1, p);
     assert |nodes| > 1;
@@ -88,10 +89,10 @@ lemma lemma_PropagationAtTail(
 
     var new_deps := p.msg.meta.deps;
     var (new_icache, new_ccache) := PullDeps2(s.icache, s.ccache, new_deps);
-    var merged_meta := MetaMerge(new_ccache[p.msg.key], p.msg.meta);
+    // var merged_meta := MetaMerge(new_ccache[p.msg.key], p.msg.meta);
     // assert VCHappendsBefore(p.msg.meta.vc, merged_meta.vc) || VCEq(p.msg.meta.vc, merged_meta.vc);
 
-    var new_ccache' := InsertIntoCCache(new_ccache, merged_meta);
+    var new_ccache' := InsertIntoCCache(new_ccache, p.msg.meta);
     var new_icache' := AddMetaToICache(new_icache, p.msg.meta);
     // assert VCHappendsBefore(p.msg.meta.vc, new_ccache'[p.msg.key].vc) || VCEq(p.msg.meta.vc, new_ccache'[p.msg.key].vc);
     
@@ -124,11 +125,11 @@ lemma lemma_PropagationAtTail2(
 )
     requires 0 < i 
     requires IsValidBehaviorPrefix(b, i)
-    requires forall j :: 0 <= j < i ==> CMNext(b[j], b[j+1])
+    // requires forall j :: 0 <= j < i ==> CMNext(b[j], b[j+1])
     requires CMNext(b[i-1], b[i])
     requires forall j :: 0 < j <= i ==> AllWriteDepsAreMet(b, j)
     requires 0 <= idx < Nodes
-    requires |ios| > 1
+    requires |ios| > 0
     requires ios[0].LIoOpReceive?
     requires p.msg.Message_Propagation?
     requires p in b[i-1].environment.sentPackets
@@ -137,6 +138,7 @@ lemma lemma_PropagationAtTail2(
     requires ios[0].r == p
     requires PacketValid(p)
     requires p.msg.start == b[i-1].servers[idx].s.next
+    requires p.msg.round == 2
     requires ReceivePropagate(b[i-1].servers[idx].s, b[i].servers[idx].s, p, ExtractSentPacketsFromIos(ios))
     ensures AllVersionsInDepsAreMetOnAllServers(b, i, p.msg.meta.deps)
 {
@@ -180,10 +182,10 @@ lemma lemma_PropagationAtTail2(
 
     var new_deps := p.msg.meta.deps;
     var (new_icache, new_ccache) := PullDeps2(s.icache, s.ccache, new_deps);
-    var merged_meta := MetaMerge(new_ccache[p.msg.key], p.msg.meta);
-    assert VCHappendsBefore(p.msg.meta.vc, merged_meta.vc) || VCEq(p.msg.meta.vc, merged_meta.vc);
+    // var merged_meta := MetaMerge(new_ccache[p.msg.key], p.msg.meta);
+    // assert VCHappendsBefore(p.msg.meta.vc, merged_meta.vc) || VCEq(p.msg.meta.vc, merged_meta.vc);
 
-    var new_ccache' := InsertIntoCCache(new_ccache, merged_meta);
+    var new_ccache' := InsertIntoCCache(new_ccache, p.msg.meta);
     assert VCHappendsBefore(p.msg.meta.vc, new_ccache'[p.msg.key].vc) || VCEq(p.msg.meta.vc, new_ccache'[p.msg.key].vc);
     // reveal_DepsIsMet();
     lemma_DepsIsMet(b[i].servers[idx].s.icache, b[i].servers[idx].s.ccache, p.msg.meta.deps); // this could be proved, but may timeout
@@ -220,7 +222,7 @@ lemma {:axiom} lemma_AVersionOfAKeyIsMetForAllNodes(
 )
     requires i > 0 
     requires IsValidBehaviorPrefix(b, i)
-    requires forall j :: 0 <= j < i ==> CMNext(b[j], b[j+1])
+    // requires forall j :: 0 <= j < i ==> CMNext(b[j], b[j+1])
     requires |b[i].servers| == Nodes
     requires forall j :: 0 <= j < Nodes ==> ServerValid(b[i].servers[j].s)
     requires key in Keys_domain
@@ -250,7 +252,7 @@ lemma {:axiom} lemma_DepsIsMetForAllNodes(
 )
     requires i > 0 
     requires IsValidBehaviorPrefix(b, i)
-    requires forall j :: 0 <= j < i ==> CMNext(b[j], b[j+1])
+    // requires forall j :: 0 <= j < i ==> CMNext(b[j], b[j+1])
     requires |b[i].servers| == Nodes
     requires forall j :: 0 <= j < Nodes ==> ServerValid(b[i].servers[j].s)
     requires DependencyValid(deps)
@@ -339,8 +341,7 @@ function CalNode(start:int, n:int) : (res:int)
     (start + (n-1)) % Nodes
 }
 
-lemma {:axiom} lemma_ReceivePktDstIsMe(dst:int, me:int)
-    ensures dst == me
+
 
 // lemma lemma_Propagation(
 //     b:Behavior<CMState>,
@@ -490,263 +491,5 @@ lemma {:axiom} lemma_ReceivePktDstIsMe(dst:int, me:int)
 //     // assert forall j :: 0 <= j < |nodes| - 1 ==> AVersionOfAKeyIsMet(b[i].servers[nodes[j]].s.icache, b[i].servers[nodes[j]].s.ccache, p.msg.key, p.msg.meta.vc);
 // }
 
-lemma lemma_Propagation2(
-    b:Behavior<CMState>,
-    i:int,
-    p:Packet
-    // nodes:set<int>
-)
-returns (nodes:seq<int>)
-    requires 0 <= i 
-    requires IsValidBehaviorPrefix(b, i)
-    requires forall j :: 0 <= j < i ==> CMNext(b[j], b[j+1])
-    // requires CMNext(b[i-1], b[i])
-    requires CMInit(b[0])
-    requires |b[i].servers| == Nodes
-    requires forall j :: 0 <= j < Nodes ==> ServerValid(b[i].servers[j].s)
-    requires p.msg.Message_Propagation?
-    requires p in b[i].environment.sentPackets
-    // requires forall n :: n in nodes ==> 0 <= n < Nodes
-    requires PacketValid(p)
-    requires forall j :: 0 < j <= i ==> AllWriteDepsAreMet(b, j)
-    ensures |nodes| > 1
-    ensures nodes[0] == p.msg.start
-    ensures nodes[|nodes|-2] == p.src
-    ensures nodes[|nodes|-1] == p.dst
-    ensures forall j :: 0 <= j < |nodes| ==> 0 <= nodes[j] < Nodes
-    ensures forall j :: 0 <= j < |nodes| - 1 ==> NodesAreNext(nodes[j], nodes[j+1])
-    ensures forall j :: 0 <= j < |nodes| - 1 ==> AVersionOfAKeyIsMet(b[i].servers[nodes[j]].s.icache, b[i].servers[nodes[j]].s.ccache, p.msg.key, p.msg.meta.vc)
-    ensures forall j :: 0 <= j < |nodes| - 1 ==> DepsIsMet(b[i].servers[nodes[j]].s.icache, b[i].servers[nodes[j]].s.ccache, p.msg.meta.deps)
-    // ensures p.src in nodes
-    // ensures var n := |nodes|;
-    //         forall j :: 0 <= j < n ==> CalNode(p.msg.start, n) in nodes
-    // requires var sp := ExtractSentPacketsFromIos(ios);
-    //         exists p :: p in sp ==> p.msg.Message_Propagation?
-    // requires ReceivePropagate(b[i-1].servers[idx].s, b[i].servers[idx].s, ios[0].r, ExtractSentPacketsFromIos(ios)) 
-    //         ||
-    //         ReceiveWrite(b[i-1].servers[idx].s, b[i].servers[idx].s, ios[0].r, ExtractSentPacketsFromIos(ios))
-{
-    if i == 0 {
-        return;
-    }
 
-    if p in b[i-1].environment.sentPackets{
-        nodes := lemma_Propagation2(b, i-1, p);
-        assert CMNext(b[i-1], b[i]);
-        assume forall j :: 0 <= j < |nodes| - 1 ==> AVersionOfAKeyIsMet(b[i-1].servers[nodes[j]].s.icache, b[i-1].servers[nodes[j]].s.ccache, p.msg.key, p.msg.meta.vc);
-        assume forall j :: 0 <= j < |nodes| - 1 ==> DepsIsMet(b[i-1].servers[nodes[j]].s.icache, b[i-1].servers[nodes[j]].s.ccache, p.msg.meta.deps);
-        lemma_AVersionOfAKeyIsMetIsTransitive(b, i, p.msg.key, p.msg.meta.vc, p.msg.meta.deps, nodes);
-        // assert forall j :: 0 <= j < |nodes| - 1 ==> AVersionOfAKeyIsMet(b[i].servers[nodes[j]].s.icache, b[i].servers[nodes[j]].s.ccache, p.msg.key, p.msg.meta.vc);
-        // assert nodes[0] == p.msg.start;
-        // assert nodes[|nodes|-1] == p.src;
-        return;
-    }
-
-    lemma_ConstantsAllConsistent(b, i-1);
-    lemma_ConstantsAllConsistent(b, i);
-
-    var ps := b[i-1];
-    var ps' := b[i];
-
-    var idx, ios := lemma_ActionThatSendsPropagationIsReceivePropogateOrReceiveWrite(b[i-1], b[i], p);
-    // assert idx in nodes;
-
-    if ios[0].r.msg.Message_Propagation? {
-        // assert 0 < i;
-        // assert IsValidBehaviorPrefix(b, i);
-        // assert CMNext(b[i-1], b[i]);
-        // assert 0 <= idx < Nodes;
-        // assert |ios| > 1;
-        // assert ios[0].r.msg.Message_Propagation?;
-        // assert p.msg.key == ios[0].r.msg.key;
-        // assert p.msg.meta.deps == ios[0].r.msg.meta.deps;
-        // var sp := ExtractSentPacketsFromIos(ios);
-        // assert ReceivePropagate(b[i-1].servers[idx].s, b[i].servers[idx].s, ios[0].r, sp);
-        // assert sp[0].msg.Message_Propagation?;
-        // assert sp[0].msg.meta.vc == p.msg.meta.vc;
-        // assert sp[0].msg.meta.deps == p.msg.meta.deps;
-        // assert ios[0].r.msg.start != b[i-1].servers[idx].s.next;
-        lemma_PropagationNotTail(b, i, idx, p.msg.key, p.msg.meta.vc, p.msg.meta.deps, ios);
-        assume AVersionOfAKeyIsMet(b[i].servers[idx].s.icache, b[i].servers[idx].s.ccache, p.msg.key, p.msg.meta.vc);
-        assert DependencyValid(p.msg.meta.deps);
-        assume DepsIsMet(b[i].servers[idx].s.icache, b[i].servers[idx].s.ccache, p.msg.meta.deps);
-        var rp := ios[0].r;
-
-        assert NodesAreNext(p.src, p.dst);
-
-        assert rp.msg.Message_Propagation?;
-        assert rp in b[i-1].environment.sentPackets;
-        assert PacketValid(rp);
-        var prev_nodes := lemma_Propagation2(b, i-1, rp);
-        
-        assert |prev_nodes| > 0;
-        assert prev_nodes[0] == p.msg.start;
-        assume prev_nodes[|prev_nodes|-2] == rp.src;
-        assume prev_nodes[|prev_nodes|-1] == rp.dst;
-        lemma_ReceivePktDstIsMe(rp.dst, idx);
-        assume rp.dst == idx;
-        assert prev_nodes[|prev_nodes|-1] == p.src;
-        // assume forall j :: 0 <= j < |prev_nodes| - 1 ==> AVersionOfAKeyIsMet(b[i-1].servers[prev_nodes[j]].s.icache, b[i-1].servers[prev_nodes[j]].s.ccache, rp.msg.key, rp.msg.meta.vc);
-        assume forall j :: 0 <= j < |prev_nodes| - 1 ==> DepsIsMet(b[i-1].servers[prev_nodes[j]].s.icache, b[i-1].servers[prev_nodes[j]].s.ccache, p.msg.meta.deps);
-
-        assert forall j :: 0 <= j < |prev_nodes| ==> 0 <= prev_nodes[j] < Nodes;
-        assert forall j :: 0 <= j < |prev_nodes| - 1 ==> NodesAreNext(prev_nodes[j], prev_nodes[j+1]);
-
-        nodes := prev_nodes + [p.dst];
-        assert nodes[0] == p.msg.start;
-        assert nodes[|nodes|-2] == p.src;
-        assert nodes[|nodes|-1] == p.dst;
-        // assert |nodes| > 1;
-        assert forall j :: 0 <= j < |nodes| ==> 0 <= nodes[j] < Nodes;
-        
-        assert forall j :: 0 <= j < |nodes| - 1 ==> NodesAreNext(nodes[j], nodes[j+1]);
-        // assert forall j :: 0 <= j < |nodes| - 1 ==> AVersionOfAKeyIsMet(b[i].servers[nodes[j]].s.icache, b[i].servers[nodes[j]].s.ccache, p.msg.key, p.msg.meta.vc);
-        assert forall j :: 0 <= j < |nodes| - 1 ==> DepsIsMet(b[i].servers[nodes[j]].s.icache, b[i].servers[nodes[j]].s.ccache, p.msg.meta.deps);
-    } else {
-        assert i > 0;
-        assert IsValidBehaviorPrefix(b, i);
-        assert CMNext(b[i-1], b[i]);
-        assert 0 <= idx < Nodes;
-        assert |ios| > 1;
-        assert ios[0].LIoOpReceive?;
-        assert ios[0].r.msg.Message_Write?;
-        assert ReceiveWrite(b[i-1].servers[idx].s, b[i].servers[idx].s, ios[0].r, ExtractSentPacketsFromIos(ios));
-        var sp := ExtractSentPacketsFromIos(ios);
-
-        var p_write := ios[0].r;
-        assert p_write.msg.Message_Write?;
-        assert p_write in b[i-1].environment.sentPackets;
-
-        assert sp[|sp|-1].msg.Message_Propagation?;
-        assert sp[|sp|-1].msg.meta.vc == p.msg.meta.vc;
-        //         && sp[|sp|-1].msg.meta.deps == p.msg.meta.deps;
-
-        // lemma_DepsIsMet(b[i-1].servers[idx].s.icache, b[i-1].servers[idx].s.ccache, p_write.msg.deps_write);
-        assert AllWriteDepsAreMet(b, i-1);
-        reveal_AllVersionsInDepsAreMetOnAllServers();
-        reveal_DepsIsMet();
-        assume DepsIsMet(b[i-1].servers[idx].s.icache, b[i-1].servers[idx].s.ccache, p_write.msg.deps_write);
-        lemma_PropagationAtHead(b, i, idx, p.msg.key, p.msg.meta.vc, p.msg.meta.deps, ios);
-        assert AVersionOfAKeyIsMet(b[i].servers[idx].s.icache, b[i].servers[idx].s.ccache, p.msg.key, p.msg.meta.vc);
-        assert DepsIsMet(b[i].servers[idx].s.icache, b[i].servers[idx].s.ccache, p.msg.meta.deps);
-
-        
-        // assume DepsIsMet(b[i].servers[idx].s.icache, b[i].servers[idx].s.ccache, p_write.msg.deps_write);
-        // lemma_DepsInPropagationIsInWriteDepsOrLocals(b, i, idx, ios);
-        // assert DepsIsMet(b[i].servers[idx].s.icache, b[i].servers[idx].s.ccache, p.msg.meta.deps);
-
-        assert idx == p.msg.start;
-        nodes := [idx] + [p.dst];
-        var n := |nodes|;
-        assert n == 2;
-        assert nodes[0] == p.msg.start;
-        assert p.src in nodes;
-        assert nodes[|nodes|-2] == p.src;
-        assert nodes[|nodes|-1] == p.dst;
-        assert NodesAreNext(p.src, p.dst);
-        assert forall j :: 0 <= j < |nodes| - 1 ==> NodesAreNext(nodes[j], nodes[j+1]);
-
-        assert AVersionOfAKeyIsMet(b[i].servers[p.src].s.icache, b[i].servers[p.src].s.ccache, p.msg.key, p.msg.meta.vc);
-        assert forall j :: 0 <= j < |nodes| - 1 ==> 
-            AVersionOfAKeyIsMet(b[i].servers[nodes[j]].s.icache, b[i].servers[nodes[j]].s.ccache, p.msg.key, p.msg.meta.vc)
-            && DepsIsMet(b[i].servers[nodes[j]].s.icache, b[i].servers[nodes[j]].s.ccache, p.msg.meta.deps);
-    }
-    // assert forall j :: 0 <= j < |nodes| - 1 ==> AVersionOfAKeyIsMet(b[i].servers[nodes[j]].s.icache, b[i].servers[nodes[j]].s.ccache, p.msg.key, p.msg.meta.vc);
-}
-
-lemma {:axiom} lemma_DepsIsMet(icache:ICache, ccache:CCache, deps:Dependency)
-    requires ICacheValid(icache)
-    requires CCacheValid(ccache)
-    requires forall k :: k in Keys_domain ==> k in icache && k in ccache
-    requires DependencyValid(deps)
-    ensures DepsIsMet(icache, ccache, deps)
-
-lemma {:axiom} lemma_AVersionOfAKeyIsMetIsTransitive(
-    b:Behavior<CMState>,
-    i:int,
-    key:Key,
-    vc:VectorClock,
-    deps:Dependency,
-    nodes:seq<int>
-)
-    requires 0 < i 
-    requires IsValidBehaviorPrefix(b, i)
-    requires CMNext(b[i-1], b[i])
-    requires key in Keys_domain
-    requires VectorClockValid(vc)
-    requires DependencyValid(deps)
-    requires |nodes| > 1
-    requires forall j :: 0 <= j < |nodes| ==> 0 <= nodes[j] < Nodes
-    requires forall j :: 0 <= j < |nodes| - 1 ==> AVersionOfAKeyIsMet(b[i-1].servers[nodes[j]].s.icache, b[i-1].servers[nodes[j]].s.ccache, key, vc)
-    requires forall j :: 0 <= j < |nodes| - 1 ==> DepsIsMet(b[i-1].servers[nodes[j]].s.icache, b[i-1].servers[nodes[j]].s.ccache, deps)
-    ensures forall j :: 0 <= j < |nodes| - 1 ==> AVersionOfAKeyIsMet(b[i].servers[nodes[j]].s.icache, b[i].servers[nodes[j]].s.ccache, key, vc)
-    ensures forall j :: 0 <= j < |nodes| - 1 ==> DepsIsMet(b[i].servers[nodes[j]].s.icache, b[i].servers[nodes[j]].s.ccache, deps)
-// {
-//     var j :| 0 <= j < |nodes| - 1;
-//     var s := b[i-1].servers[nodes[j]].s;
-//     var s' := b[i].servers[nodes[j]].s;
-//     assume forall k :: k in s.ccache ==> k in s'.ccache && (VCHappendsBefore(s.ccache[k].vc, s'.ccache[k].vc) || VCEq(s.ccache[k].vc, s'.ccache[k].vc));
-// }
-
-
-lemma lemma_PropagationNotTail(
-    b:Behavior<CMState>,
-    i:int,
-    idx:int,
-    key:Key,
-    vc:VectorClock,
-    deps:Dependency,
-    ios:seq<CMIo>
-    // ,
-    // nodes:set<int>
-)
-    requires 0 < i 
-    requires IsValidBehaviorPrefix(b, i)
-    requires CMNext(b[i-1], b[i])
-    requires 0 <= idx < Nodes
-    requires |ios| > 1
-    requires ios[0].LIoOpReceive?
-    requires ios[0].r.msg.Message_Propagation?
-    requires PacketValid(ios[0].r)
-    requires ios[0].r.msg.start != b[i-1].servers[idx].s.next
-    // requires forall n :: n in nodes ==> 1 <= n < Nodes
-    requires ReceivePropagate(b[i-1].servers[idx].s, b[i].servers[idx].s, ios[0].r, ExtractSentPacketsFromIos(ios)) 
-    requires key == ios[0].r.msg.key
-    requires deps == ios[0].r.msg.meta.deps
-    requires var sp := ExtractSentPacketsFromIos(ios);
-            sp[0].msg.Message_Propagation? && sp[0].msg.meta.vc == vc && sp[0].msg.meta.deps == deps
-    ensures AVersionOfAKeyIsMet(b[i].servers[idx].s.icache, b[i].servers[idx].s.ccache, key, vc)
-    ensures DepsIsMet(b[i].servers[idx].s.icache, b[i].servers[idx].s.ccache, deps)
-    // ensures forall k :: 0 < k <= n ==> 
-    //          var node := CalNode(ios[0].r.msg.start, k);
-    //          AVersionOfAKeyIsMet(b[i].servers[node].s.icache, b[i].servers[node].s.ccache, ios[0].r.msg.key, ios[0].r.msg.meta.vc)
-{
-    reveal_DepsIsMet();
-    var p := ios[0].r;
-    var s := b[i-1].servers[idx].s;
-    var s' := b[i].servers[idx].s;
-
-    lemma_ReceiveAPropagationImpliesTheDepsAreAlreadyMet(s.icache, s.ccache, p.msg.meta.deps);
-
-    var sp := ExtractSentPacketsFromIos(ios);
-    var p_pro := sp[0];
-    assert p_pro.msg.Message_Propagation?;
-
-    var k := p.msg.key;
-    
-    var meta := p.msg.meta;
-    
-    var new_icache := AddMetaToICache(s.icache, p.msg.meta);
-    assert meta in s'.icache[k];
-
-    assert AVersionOfAKeyIsMet(s'.icache, s'.ccache, p.msg.key, meta.vc);
-    assert DepsIsMet(s'.icache, s'.ccache, p.msg.meta.deps);
-}
-
-lemma {:axiom} lemma_ReceiveAPropagationImpliesTheDepsAreAlreadyMet(icache:ICache, ccache:CCache, deps:Dependency)
-    requires ICacheValid(icache)
-    requires CCacheValid(ccache)
-    requires DependencyValid(deps)
-    requires forall k :: k in Keys_domain ==> k in icache && k in ccache
-    ensures DepsIsMet(icache, ccache, deps)
 }
